progress in 5

Ex5.dfy
@@ -7,33 +7,163 @@ module Ex5 {
   class Set {
     var tbl : array<bool>  
     var list : Ex3.Node?
+    ghost var size : nat
+    ghost var content : set<nat>
+    ghost var footprint : set<Ex3.Node>
 
     ghost function Valid() : bool 
+    reads this, footprint, this.list, tbl
     {
-
+      if (this.list == null)
+        then 
+          footprint == {}
+          &&
+          content == {}
+          && 
+          tbl.Length == size
+          && 
+          validTable(tbl, content)
+        else 
+          footprint == list.footprint
+          &&
+          content == list.content
+          && 
+          tbl.Length == size
+          &&
+          validTable(tbl, content)
+          &&
+          list.Valid()
     }
       
-    constructor (size : nat) 
+    constructor (size : nat)
+    ensures Valid() && this.content == {} && this.footprint == {} && this.size == size
     {
+      tbl := new bool[size] (_ => false);
+      list := null;
+      footprint := {};
+      this.size := size;
+      content := {};
     }
 
 
     method mem (v : nat) returns (b : bool)
+    requires Valid() && v < size
+    ensures b == (v in content)
     {
+      if tbl[v] {
+        b := true;
+        return;
+      }
+      else {
+        b := false;
+        return;
+      }
     }
     
     method add (v : nat) 
+    requires Valid() && v < size
+    modifies this, tbl
+    ensures Valid()
+    ensures this.content == {v} + old(this.content)
+    ensures this.footprint >= old(this.footprint)
+    ensures this.footprint > old(this.footprint) ==>  fresh(this.footprint - old(this.footprint))
     {
+      if (this.list == null) {
+        var n := new Ex3.Node(v);
+        this.list := n;
+        this.tbl[v] := true;
+        this.content := {v};
+        this.footprint := {n};
+      }
+      else {
+        var condition := this.list.mem(v);
+        if (! condition) {
+          var n := this.list.add(v);
+          this.list := n;
+          this.tbl[v] := true;
+          this.content := {v} + this.content;
+          this.footprint := {n} + this.footprint;
+        }
+      }
     }
 
     method union(s : Set) returns (r : Set)
+    requires Valid() && s.Valid()
+    decreases footprint
+    ensures fresh(r) && r.Valid()
+    ensures r.content == s.content + this.content
     {
+      var max_size := max(this.tbl.Length, s.tbl.Length);
+      r := new Set(max_size);
+      var cur1 := this.list;
+      var list_aux : set<nat> := {};
+      while (cur1 != null)
+      invariant r.Valid()
+      invariant cur1 != null ==> cur1.Valid()
+      invariant r.content == list_aux
+      invariant cur1 != null ==> this.content == list_aux + cur1.content
+      invariant cur1 == null ==> list_aux == this.content
+      decreases if cur1 != null then cur1.footprint else {}
+      {
+        r.add(cur1.val);
+        list_aux := list_aux + {cur1.val};
+        cur1 := cur1.next;
+      }
+      var cur2 := s.list;
+      var list_aux2 : set<nat> := {};
+      while (cur2 != null)
+      invariant r.Valid()
+      invariant r.content == list_aux2 + content
+      invariant cur2 != null ==> cur2.Valid()
+      invariant cur2 != null ==> s.content == list_aux2 + cur2.content
+      invariant cur2 == null ==> list_aux2 == s.content
+      decreases if cur2 != null then cur2.footprint else {}
+      {
+        r.add(cur2.val);
+        list_aux2 := list_aux2 + {cur2.val};
+        cur2 := cur2.next;
+      }
     }
 
     method inter(s : Set) returns (r : Set)
+    requires Valid() && s.Valid()
+    ensures fresh(r) && r.Valid()
+    ensures r.content == s.content * this.content
     {
+      var max_size := max(this.tbl.Length, s.tbl.Length);
+      r := new Set(max_size);
+      var cur1 := this.list;
+      ghost var list_aux : set<nat> := {};
+      while (cur1 != null)
+      invariant r.Valid()
+      invariant cur1 != null ==> cur1.Valid()
+      invariant r.content == list_aux * s.content
+      invariant (cur1 != null) ==> (this.content == list_aux + cur1.content)
+      invariant (cur1 == null) ==> (list_aux == this.content)
+      decreases if cur1 != null then cur1.footprint else {}
+      {
+        var condition := s.mem(cur1.val);
+        if (condition) {
+          r.add(cur1.val);
+        }
+        list_aux := list_aux + {cur1.val};
+
+        cur1 := cur1.next;
+      }
     }
 
+  }
+
+  function validTable(tbl : array<bool>, content : set<nat>) : bool
+  reads tbl
+  {
+    forall k :: 0 <= k < tbl.Length ==> (tbl[k] == (k in content))
+  }
+
+  function max(n1 : nat, n2 : nat) : nat
+  {
+    if (n1 > n2) then n1
+    else n2
   }
 
 }
